theories/zoo_std/mpsc_waiter__opaque.v
@@ -1,6 +1,0 @@
-Require Import zoo_std.mpsc_waiter__code.
-
-#[global] Opaque mpsc_waiter٠create.
-#[global] Opaque mpsc_waiter٠notify.
-#[global] Opaque mpsc_waiter٠try_wait.
-#[global] Opaque mpsc_waiter٠wait.
