theories/zoo_std/waiter_mpsc__opaque.v
@@ -1,0 +1,6 @@
+Require Import zoo_std.waiter_mpsc__code.
+
+#[global] Opaque waiter_mpsc٠create.
+#[global] Opaque waiter_mpsc٠notify.
+#[global] Opaque waiter_mpsc٠try_wait.
+#[global] Opaque waiter_mpsc٠wait.
